substitution

Denote/PCF/Red.lean
@@ -2,45 +2,25 @@ import Denote.PCF.Stx
 
 namespace PCF
 
-def Term'.subst : Term' (Term' A) t → Term' A t
-  | .lam l => .lam fun v => (l (.var v)).subst
-  | .var v => v
-  | .app a b => .app a.subst b.subst
-
-  | .zero => .zero
-  | .false => .false
-  | .true => .true
-
-  | .succ v => .succ v.subst
-  | .fix v => .fix v.subst
-  | .z? v => .z? v.subst
-  | .pred v => .pred v.subst
-
-  | .ite c t f => .ite c.subst t.subst f.subst
-
-inductive Term'.Val : Term' A t → Prop
+inductive ITerm.Val : ITerm Γ t → Prop
   | zero : Val .zero
   | succ : Val v → Val (.succ v)
   | true : Val .true
   | false : Val .false
   | lam : Val (.lam l)
 
-def Term.Val (v : Term t) : Prop := 
-  Term'.Val (A := fun _ => PUnit) v
+inductive Red : ITerm [] t → ITerm [] t → Prop
+  | val : v.Val → Red v v
+  | succ : Red x v → Red (.succ x) (.succ v)
+  | pred : Red x (.succ v) → Red (.pred x) v
+  | z?z : Red x .zero → Red (.z? x) .true
+  | z?s : Red x (.succ _) → Red (.z? x) .false
+  | itet : Red c .true → Red t v → Red (.ite c t f) v
+  | itef : Red c .false → Red f v → Red (.ite c t f) v
+  | app : Red t (.lam f) → Red (f.parSubst <| .cons u .nil) v → Red (.app t u) v
+  | fix : Red (.app t (.fix t)) v → Red (.fix t) v
 
-inductive Red : Term t → Term t → Prop
-  | val : Term.Val v → Red v v
-  | succ : Red x v → Red (Term.succ x) (Term.succ v)
-  | pred : Red x (Term.succ v) → Red (Term.pred x) v
-  | z?z : Red x .zero → Red (Term.z? x) .true
-  | z?s : Red x (Term.succ _) → Red (Term.z? x) .false
-  | itet : Red c .true → Red t v → Red (Term.ite c t f) v
-  | itef : Red c .false → Red f v → Red (Term.ite c t f) v
-  | app {t : Term (.arr A B)} {u : Term A} {v : Term B} {f : {rep : Ty → Type} → rep A → Term B}
-      : Red t (Term.lam f) → Red (f u).subst v → Red (Term.app t u) v
-  | fix : Red (Term.app t (Term.fix t)) v → Red (Term.fix t) v
-
-theorem Red.rhs_Val (h : Red a b) : Term.Val b := by
+theorem Red.rhs_Val (h : Red a b) : b.Val := by
   induction h
   any_goals assumption
   case succ ih => exact .succ ih
@@ -48,5 +28,5 @@ theorem Red.rhs_Val (h : Red a b) : Term.Val b := by
   case z?z => exact .true
   case z?s => exact .false
 
-def Ω (t : Ty) : Term t := .fix <| .lam fun x => .var x
+def Ω Γ t : ITerm Γ t := .fix <| .lam <| .var .hd
 
