Denote/PCF/Approx.lean
@@ -1,0 +1,23 @@
+import Denote.PCF.Red
+import Denote.PCF.Denote
+
+namespace PCF
+
+def ITerm.ofNat : (n : Nat) → ITerm Γ .nat
+  | 0 => .zero
+  | n+1 => .succ <|.ofNat n
+
+instance {Γ} {n : Nat} : OfNat (ITerm Γ .nat) n where
+  ofNat := ITerm.ofNat n
+
+def Approx : {t : Ty} → t.denote → ITerm [] t → Prop
+  | .bool, .bot, _ | .nat, .bot, _ => True
+  | .nat, .obj n, t => Red t (.ofNat n)
+  | .bool, .obj .true, t => Red t .true
+  | .bool, .obj .false, t => Red t .false
+  | .arr _ _, d, t => ∀ e u, Approx e u → Approx (d.f (e)) (.app t u)
+
+
+
+end PCF
+
