Denote/PCF/Subst.lean
@@ -1,0 +1,151 @@
+import Denote.PCF.Stx
+import Denote.PCF.Red
+import Denote.PCF.Denote
+import Denote.PCF.DenoteDefs
+import Denote.Domain.Flat
+import Denote.Domain.FuncDom
+import Denote.Domain.DomConstructs
+
+namespace PCF
+
+open Dom
+
+noncomputable section
+def deepApply (h : ctx_denote Γ₂) : {Γ : _}
+    → HList (ITerm Γ₂) Γ
+    → ctx_denote Γ
+  | _, .nil => .unit
+  | _, .cons hd tl => ⟨deepApply h tl, hd.denote h⟩
+
+def ctx_denote.concat
+    : {a b : _}
+    → (ha : ctx_denote a)
+    → (hb : ctx_denote b)
+    → ctx_denote (a ++ b)
+  | [], _, _, hb => hb
+  | _ :: _, _, ⟨htl, hhd⟩, hb => ⟨htl.concat hb, hhd⟩
+
+theorem shift {Δ₁ : ctx_denote Γ₁}
+    : {Γ : _}
+    → {Δ : ctx_denote Γ}
+    → (v : List.MemT t (Γ₁))
+    → (proj v.shift).f (Δ.concat Δ₁) = (proj v).f Δ₁ 
+  | [], _, h => rfl
+  | _ :: _, ⟨Δ, _⟩, h => by 
+    change (proj h.shift).f (Δ.concat Δ₁) = (proj h).f Δ₁
+    exact shift h
+
+theorem sshift {Δ₁ : ctx_denote Γ₁}
+    : {Γ Γ₂ : _}
+    → {Δ : ctx_denote Γ}
+    → {Δ₂ : ctx_denote Γ₂}
+    → (v : List.MemT t (Γ ++ Γ₁))
+    → (proj v.sandwitch_shift).f (Δ.concat (Δ₂.concat Δ₁)) = (proj v).f (Δ.concat Δ₁)
+  | [], _, .unit, _, v => shift v
+  | _ :: _, _, ⟨_, _⟩, _, .hd => rfl
+  | _ :: _, _, ⟨_, _⟩, _, .tl h => sshift h
+
+theorem gshift {Γ Γ₁ Γ₂} {Δ Δ₁ Δ₂ : ctx_denote.{u} _}
+    : {a : ITerm (Γ ++ Γ₁) t} 
+    → (ITerm.gshift (Γ₂ := Γ₂) a).denote.f (.concat Δ (.concat Δ₂ Δ₁)) = a.denote (.concat Δ Δ₁)
+  | .var v => by
+    simp only [Ty.denote, Function.comp_apply, ITerm.gshift, ITerm.denote]
+    exact sshift v
+  | .z? v
+  | .pred v
+  | .succ v
+  | .ite c t f
+  | .app a b
+  | .fix v => by
+    unfold ITerm.gshift
+    dsimp [ITerm.denote, CFunc.comp, CFunc.corecP, Prod.corec]
+    repeat rw [gshift]
+  | .false | .zero | .true => by simp [ITerm.gshift, ITerm.denote, CFunc.const]
+  | .lam (dom := dom) a => by
+    unfold ITerm.gshift
+    apply CFunc.ext
+    funext v
+    exact gshift (Γ := dom :: Γ) (Δ := ⟨Δ,v⟩)
+
+theorem shift1 {Γ₁} {Δ : ctx_denote _}
+    {a : ITerm Γ₁ t}
+    : (ITerm.shift [t₂] a).denote.f (Δ, v) = a.denote Δ :=
+  @gshift t [] Γ₁ [t₂] .unit Δ ⟨.unit, v⟩ a
+
+theorem deepApply_denote
+    (Δ : ctx_denote Γ₂)
+    : {Γ : _}
+    → (Δ' : HList (ITerm Γ₂) Γ)
+    → (h : List.MemT t₂ Γ)
+    → Δ'[h].denote.f Δ = (proj h).f (deepApply Δ Δ')
+  | _ :: _, .cons _ _, .hd => rfl
+  | _ :: _, .cons _ tl, .tl h => 
+    deepApply_denote Δ tl h
+
+theorem subst
+    {Δ' : HList (ITerm Γ₂) Γ}
+    : {t : ITerm Γ t₂} → (t.parSubst Δ').denote Δ = t.denote (deepApply Δ Δ')
+  | .var h => by
+    dsimp [ITerm.parSubst, ITerm.denote]
+    apply deepApply_denote
+  | .false | .true | .zero => rfl
+  | .fix v => by
+    change ((v.parSubst _).denote Δ).fix' = (v.denote.f _).fix'
+    rw [subst]
+  | .z? v => by
+    change z?.denote ((v.parSubst _).denote Δ) = z?.denote _
+    rw [subst]
+  | .pred v => by
+    change pred.denote ((v.parSubst _).denote Δ) = pred.denote _
+    rw [subst]
+  | .succ v => by
+    change succ.denote ((v.parSubst _).denote Δ) = succ.denote _
+    rw [subst]
+  | .ite c t f => by
+    change ite.denote ⟨
+      (c.parSubst _).denote Δ,
+      (t.parSubst _).denote Δ,
+      (f.parSubst _).denote Δ
+    ⟩ = ite.denote ⟨_,_,_⟩
+    rw [subst, subst, subst]
+  | .app a b => by
+    change CFunc.mp ⟨
+      (a.parSubst _).denote Δ,
+      (b.parSubst _).denote Δ
+    ⟩ = CFunc.mp ⟨a.denote _, b.denote _⟩
+    rw [subst, subst]
+  | .lam l => by
+    apply CFunc.ext
+    funext v
+    change (ITerm.parSubst (HList.cons (ITerm.var List.MemT.hd) _) l).denote.f (Δ, v) = 
+      l.denote.f (deepApply Δ Δ', v)
+    rw [subst]
+    congr
+    refine Prod.ext ?_ rfl
+    dsimp [deepApply, ITerm.denote, proj]
+    clear *-
+    induction Δ'
+    · rfl
+    case cons ih =>
+      dsimp [deepApply, HList.map]
+      apply Prod.ext
+      · exact ih
+      · rw [shift1]
+
+/- theorem shift1 {dom v} : {a : ITerm Γ t} → (ITerm.shift [dom] a).denote.f (Δ, v) = a.denote Δ -/
+/-   | .var _ => sorry -/
+/-   | .fix _ => sorry -/
+/-   | .z? _ => sorry -/
+/-   | .pred _ => sorry -/
+/-   | .succ _ => sorry -/
+/-   | .zero => sorry -/
+/-   | .ite _ _ _ => sorry -/
+/-   | .false => sorry -/
+/-   | .true => sorry -/
+/-   | .app _ _ => sorry -/
+/-   | .lam _ => sorry -/
+
+end
+
+end PCF
+
